Some more BST proofs, but not too many.

DS/BST.v
@@ -76,50 +76,222 @@ match t with
         end
 end.
 
+(*
+Class TotalPreordDec : Type :=
+{
+    carrier : Type;
+    lt : carrier -> carrier -> Prop;
+    lt_antirefl :
+      forall x : carrier, ~ lt x x;
+    lt_trans :
+      forall x y z : carrier, lt x y -> lt y z -> lt x z;
+    
+}.
+*)
+(*
+Class cmp_spec {A : Type} (cmp : A -> A -> comparison) : Prop :=
+{
+    cmp_spec1 :
+      forall x y : A, cmp x y = Eq -> x = y;
+    cmp_spec2 :
+      forall x y : A, cmp x y = Lt <-> cmp y x = Gt;
+    cmp_spec3 :
+      forall x : A, cmp x x = Eq;
+}.
+*)
+Class cmp_spec (A : Type) : Type :=
+{
+    cmpr : A -> A -> comparison;
+    cmp_spec1 :
+      forall x y : A, cmpr x y = Eq -> x = y;
+    cmp_spec2 :
+      forall x y : A, cmpr x y = Lt <-> cmpr y x = Gt;
+    cmp_spec3 :
+      forall x : A, cmpr x x = Eq;
+}.
+
+Coercion cmpr : cmp_spec >-> Funclass.
+
+(*
+Class BSTOrd : Type :=
+{
+    carrier : Type;
+    cmpr : carrier -> carrier -> comparison;
+    spec : cmp_spec cmpr;
+}.
+*)
+
+Hint Extern 0 =>
+  intros;
+match goal with
+    | H : Elem _ empty |- _ => inversion H
+    | H : isBST _ (node _ ?l _) |- isBST _ ?l => inversion H; auto
+    | H : isBST _ (node _ _ ?r) |- isBST _ ?r => inversion H; auto
+end.
+
+Lemma Elem_insert :
+  forall
+    {A : Type} {cmp : cmp_spec A}
+    (x y : A) (t : BTree A),
+      isBST cmp t -> Elem x (insert cmp y t) -> x = y \/ Elem x t.
+Proof.
+  intros A cmp x y t H.
+  functional induction (insert cmp y t).
+    inversion 1; subst; auto.
+    inversion H; subst. inversion 1; firstorder.
+    inversion 1; firstorder.
+    inversion H; subst. inversion 1; subst; firstorder.
+Qed.
+
+Lemma Elem_removeMin :
+  forall
+    {A : Type} {cmp : cmp_spec A}
+    (x m : A) (t t' : BTree A),
+      isBST cmp t -> removeMin cmp t = Some (m, t') ->
+        Elem x t <-> x = m \/ x <> m /\ Elem x t'.
+Proof.
+  intros A cmp x m t t' H.
+  revert x m t' H.
+  functional induction (removeMin cmp t); intros.
+    inversion H0.
+    inversion H0; subst. split; inversion 1; subst.
+      left. reflexivity.
+      destruct l; cbn in *.
+        inversion H3.
+        destruct (removeMin cmp l1) as [[] |]; inversion e0.
+      right. split.
+        intro. inversion H; subst. specialize (H10 _ H3).
+          rewrite cmp_spec3 in H10. congruence.
+        assumption.
+      constructor.
+      destruct H2, H1 as [H11 | [H11 H12]]; auto.
+    inversion H0; subst; clear H0. split; inversion 1; subst; auto.
+Abort.
+(*
+      inversion H; subst. destruct (IHo x0 _ _ H5 e0).
+        destruct (H1 H2); auto.
+      inversion H; subst. specialize (IHo x _ _ H4 e0).
+      destruct l; cbn in *.
+        inversion e0.
+        destruct (removeMin cmp l1) as [[] |]; inversion e0; subst.
+          
+      inversion H; subst. destruct (IHo x _ _ H4 e0).
+        destruct (H1 
+*)
+
+Lemma Elem_remove :
+  forall
+    {A : Type} (cmp : cmp_spec A)
+    (x y : A) (t : BTree A),
+      isBST cmp t -> Elem x (remove cmp y t) -> x <> y /\ Elem x t.
+Proof.
+Admitted.
+
+Lemma isBST_insert :
+  forall
+    {A : Type} {cmp : cmp_spec A} (x : A) (t : BTree A),
+    isBST cmp t -> isBST cmp (insert cmp x t).
+Proof.
+  intros.
+  functional induction (insert cmp x t).
+    auto.
+    constructor; auto; intros.
+      inversion H; subst. destruct (Elem_insert _ _ _ H4 H0); subst.
+        assumption.
+        apply H5. assumption.
+      inversion H; subst. apply H7. assumption.
+    apply cmp_spec1 in e0. subst. assumption.
+    constructor; auto; intros.
+      inversion H; subst. apply H5. assumption.
+      inversion H; subst. destruct (Elem_insert _ _ _ H6 H0); subst.
+        assumption.
+        apply H7. assumption.
+Qed.
+
+Lemma isBST_removeMin :
+  forall
+    {A : Type} (cmp : cmp_spec A)
+    (t t' : BTree A) (x : A),
+      isBST cmp t -> removeMin cmp t = Some (x, t') -> isBST cmp t'.
+Proof.
+  intros. revert t' x H0.
+  functional induction (removeMin cmp t); intros.
+    inversion H0.
+    inversion H0; subst. inversion H; subst. assumption.
+    inversion H0; subst. inversion H; subst.
+      specialize (IHo H4 l' x0 e0). constructor; auto.
+        intros. apply H5. admit.
+Admitted.
+
+Lemma isBST_remove :
+  forall (A : Type) (cmp : cmp_spec A) (x : A) (t : BTree A),
+    isBST cmp t -> isBST cmp (remove cmp x t).
+Proof.
+  intros.
+  functional induction (remove cmp x t); auto.
+    constructor; auto; intros.
+      inversion H; subst. destruct (Elem_remove cmp _ _ _ H4 H0).
+        apply H5. assumption.
+      inversion H; subst. apply H7. assumption.
+    constructor; auto; intros.
+      inversion H; subst. apply H5. assumption.
+      inversion H; subst. destruct (Elem_remove cmp _ _ _ H6 H0).
+        apply H7. assumption.
+    inversion H; subst. constructor; auto; intros.
+      eapply isBST_removeMin.
+        exact H3.
+        apply e1.
+Abort.
+
 Lemma elem_spec :
-  forall {A : Type} (cmp : A -> A -> comparison) (x : A) (t : BTree A),
-    (forall x y : A, CompareSpec (x = y) (cmp x y = Lt) (cmp x y = Gt) (cmp x y)) ->
+  forall
+    {A : Type} (cmp : cmp_spec A)
+    (x : A) (t : BTree A),
       isBST cmp t -> BoolSpec (Elem x t) (~ Elem x t) (elem cmp x t).
 Proof.
-  intros A cmp x t spec H.
+  intros A cmp x t H.
   functional induction (elem cmp x t).
     constructor. inversion 1.
     inversion H; subst. specialize (IHb H3). destruct IHb.
       constructor. constructor 2. assumption.
       constructor. inversion 1; subst.
-        admit.
+        rewrite cmp_spec3 in e0. congruence.
         contradiction.
         specialize (H6 _ H7). congruence.
-    constructor. destruct (spec x v); try congruence; subst. constructor.
+    constructor. apply cmp_spec1 in e0. subst. constructor.
     inversion H; subst. specialize (IHb H5). destruct IHb.
       constructor. constructor 3. assumption.
       constructor. inversion 1; subst.
-        admit.
+        rewrite cmp_spec3 in e0. congruence.
         specialize (H4 _ H7). congruence.
         contradiction.
-Admitted.
+Qed.
 
 Lemma elem_insert :
-  forall {A : Type} (cmp : A -> A -> comparison) (x : A) (t : BTree A),
-    isBST cmp t -> elem cmp x (insert cmp x t) = true.
+  forall
+    {A : Type} (cmp : cmp_spec A)
+    (x : A) (t : BTree A),
+      isBST cmp t -> elem cmp x (insert cmp x t) = true.
 Proof.
-  intros.
+  intros A cmp x t H.
   functional induction (insert cmp x t); cbn.
-    admit.
+    rewrite cmp_spec3. reflexivity.
     rewrite e0, IHb.
       reflexivity.
       inversion H; assumption.
-    admit.
+    rewrite cmp_spec3. reflexivity.
     rewrite e0, IHb.
       reflexivity.
       inversion H; assumption.
-Admitted.
+Qed.
 
 Lemma elem_remove :
-  forall (A : Type) (cmp : A -> A -> comparison) (x : A) (t : BTree A),
-    isBST cmp t -> elem cmp x (remove cmp x t) = false.
+  forall
+    {A : Type} (cmp : cmp_spec A)
+    (x : A) (t : BTree A),
+      isBST cmp t -> elem cmp x (remove cmp x t) = false.
 Proof.
-  intros.
+  intros A cmp x t H.
   functional induction (remove cmp x t); cbn.
     reflexivity.
     rewrite e0, IHb.
@@ -128,8 +300,12 @@ Proof.
     rewrite e0, IHb.
       reflexivity.
       inversion H; assumption.
-    inversion H; subst.
-      admit.
+    inversion H; subst. destruct (elem_spec cmp x r).
+      inversion H; assumption.
+      specialize (H6 _ H0). apply cmp_spec1 in e0. subst.
+        rewrite cmp_spec3 in H6. congruence.
+      reflexivity.
+    apply cmp_spec1 in e0. subst.
 Abort.
 
 Lemma elem_insert' :
@@ -166,59 +342,6 @@ Proof.
       reflexivity.
     destruct (cmp x m) eqn: Hxm, (cmp x v) eqn: Hxv.
       all: try reflexivity.
-Admitted.
-
-Hint Extern 0 =>
-  intros;
-match goal with
-    | H : Elem _ empty |- _ => inversion H
-    | H : isBST _ (node _ ?l _) |- isBST _ ?l => inversion H; auto
-    | H : isBST _ (node _ _ ?r) |- isBST _ ?r => inversion H; auto
-end.
-
-Lemma isBST_insert :
-  forall (A : Type) (cmp : A -> A -> comparison) (x : A) (t : BTree A),
-    isBST cmp t -> isBST cmp (insert cmp x t).
-Proof.
-  intros.
-  functional induction (insert cmp x t).
-    auto.
-    constructor; auto; intros.
-      admit.
-      inversion H; subst. apply H7. assumption.
-    admit.
-    constructor; auto; intros.
-      inversion H; subst. apply H5. assumption.
-      inversion H; subst. admit.
-Admitted.
-
-Lemma isBST_remove :
-  forall (A : Type) (cmp : A -> A -> comparison) (x : A) (t : BTree A),
-    isBST cmp t -> isBST cmp (remove cmp x t).
-Proof.
-  intros.
-  functional induction (remove cmp x t); auto.
-    constructor; auto; intros.
-      admit.
-      inversion H; subst. apply H7. assumption.
-    constructor; auto; intros.
-      inversion H; subst. apply H5. assumption.
-      admit.
-    constructor; auto; intros.
-      admit.
-Abort.
-
-Lemma isBST_removeMin :
-  forall (A : Type) (cmp : A -> A -> comparison) (t t' : BTree A) (x : A),
-    isBST cmp t -> removeMin cmp t = Some (x, t') -> isBST cmp t'.
-Proof.
-  intros. revert t' x H0.
-  functional induction (removeMin cmp t); intros.
-    inversion H0.
-    inversion H0; subst. inversion H; subst. assumption.
-    inversion H0; subst. inversion H; subst.
-      specialize (IHo H4 l' x0 e0). constructor; auto.
-        intros. apply H5. admit.
 Admitted.
 
 (* TODO theorems:
